Examples.thy
@@ -2,8 +2,71 @@ theory Examples
 imports DerivedCombinators PartialEvaluation
 begin
 
-definition length_expr :: "type \<Rightarrow> expr" ("length\<^bsub>_\<^esub>")where
+definition is_zero_expr :: expr where
+  "is_zero_expr = \<epsilon> \<bar> \<kappa> UnitV \<cdot> \<prec>\<^bsub>NatF\<^esub>"
+
+definition pred_expr :: expr where
+  "pred_expr = \<kappa> ZeroV \<nabla> \<epsilon> \<cdot> \<prec>\<^bsub>NatF\<^esub>"
+
+definition greater_than_helper :: expr where
+  "greater_than_helper = 
+      IF is_zero_expr \<cdot> \<pi>\<^sub>1 THEN \<iota>\<^sub>l \<cdot> \<kappa> FalseV 
+      ELSE IF is_zero_expr \<cdot> \<pi>\<^sub>2 THEN \<iota>\<^sub>l \<cdot> \<kappa> TrueV 
+      ELSE \<iota>\<^sub>r \<cdot> pred_expr \<parallel> pred_expr 
+      FI FI"
+
+definition greater_than_expr :: expr where
+  "greater_than_expr = \<lparr> \<Xi> \<rparr>\<^bsub>K Bool \<Oplus> Id\<^esub> \<cdot> \<lbrakk> greater_than_helper \<rbrakk>\<^bsub>K Bool \<Oplus> Id\<^esub>"
+
+definition length_expr :: "type \<Rightarrow> expr" ("length\<^bsub>_\<^esub>") where
   "length\<^bsub>t\<^esub> = \<lparr> \<kappa> ZeroV \<nabla> (succ \<cdot> \<pi>\<^sub>2) \<rparr>\<^bsub>ListF t\<^esub>"
+
+lemma [simp]: "is_zero_expr \<turnstile> Nat \<rightarrow> Bool"
+  proof (unfold is_zero_expr_def)
+    have "\<prec>\<^bsub>NatF\<^esub> \<turnstile> Nat \<rightarrow> Nat \<star> NatF" by (metis tc_outj)
+    hence "\<prec>\<^bsub>NatF\<^esub> \<turnstile> Nat \<rightarrow> \<one> \<oplus> Nat" by simp
+    moreover have "\<epsilon> \<bar> \<kappa> UnitV \<turnstile> \<one> \<oplus> Nat \<rightarrow> Bool" by simp
+    ultimately show "\<epsilon> \<bar> \<kappa> UnitV \<cdot> \<prec>\<^bsub>NatF\<^esub> \<turnstile> Nat \<rightarrow> Bool" by (metis tc_comp)
+  qed
+
+lemma [simp]: "pred_expr \<turnstile> Nat \<rightarrow> Nat"
+  proof (unfold pred_expr_def)
+    have "\<prec>\<^bsub>NatF\<^esub> \<turnstile> Nat \<rightarrow> Nat \<star> NatF" by (metis tc_outj)
+    hence "\<prec>\<^bsub>NatF\<^esub> \<turnstile> Nat \<rightarrow> \<one> \<oplus> Nat" by simp
+    moreover have "\<kappa> ZeroV \<nabla> \<epsilon> \<turnstile> \<one> \<oplus> Nat \<rightarrow> Nat" by simp
+    ultimately show "\<kappa> ZeroV \<nabla> \<epsilon> \<cdot> \<prec>\<^bsub>NatF\<^esub> \<turnstile> Nat \<rightarrow> Nat" by (metis tc_comp)
+  qed
+
+lemma [simp]: "greater_than_helper \<turnstile> Nat \<otimes> Nat \<rightarrow> Bool \<oplus> Nat \<otimes> Nat"
+  proof (unfold greater_than_helper_def)
+    have E: "is_zero_expr \<turnstile> Nat \<rightarrow> Bool" by simp
+    moreover have "\<pi>\<^sub>1 \<turnstile> Nat \<otimes> Nat \<rightarrow> Nat" by simp
+    ultimately have X: "is_zero_expr \<cdot> \<pi>\<^sub>1 \<turnstile> Nat \<otimes> Nat \<rightarrow> Bool" by (metis tc_comp)
+    have I: "\<iota>\<^sub>l \<turnstile> Bool \<rightarrow> Bool \<oplus> Nat \<otimes> Nat" by simp
+    moreover have "\<kappa> FalseV \<turnstile> Nat \<otimes> Nat \<rightarrow> Bool" by simp
+    ultimately have Y: "\<iota>\<^sub>l \<cdot> \<kappa> FalseV \<turnstile> Nat \<otimes> Nat \<rightarrow> Bool \<oplus> Nat \<otimes> Nat" by (metis tc_comp)
+    have "\<pi>\<^sub>2 \<turnstile> Nat \<otimes> Nat \<rightarrow> Nat" by simp
+    with E have Z: "is_zero_expr \<cdot> \<pi>\<^sub>2 \<turnstile> Nat \<otimes> Nat \<rightarrow> Bool" by (metis tc_comp)
+    have "\<kappa> TrueV \<turnstile> Nat \<otimes> Nat \<rightarrow> Bool" by simp
+    with I have W: "\<iota>\<^sub>l \<cdot> \<kappa> TrueV  \<turnstile> Nat \<otimes> Nat \<rightarrow> Bool \<oplus> Nat \<otimes> Nat" by (metis tc_comp)
+    have "pred_expr \<parallel> pred_expr \<turnstile> Nat \<otimes> Nat \<rightarrow> Nat \<otimes> Nat" by simp
+    moreover have "\<iota>\<^sub>r \<turnstile> Nat \<otimes> Nat \<rightarrow> Bool \<oplus> Nat \<otimes> Nat" by simp
+    ultimately have "\<iota>\<^sub>r \<cdot> pred_expr \<parallel> pred_expr \<turnstile> Nat \<otimes> Nat \<rightarrow> Bool \<oplus> Nat \<otimes> Nat" by (metis tc_comp)
+    with X Y Z W show "
+      IF is_zero_expr \<cdot> \<pi>\<^sub>1 THEN \<iota>\<^sub>l \<cdot> \<kappa> FalseV 
+      ELSE IF is_zero_expr \<cdot> \<pi>\<^sub>2 THEN \<iota>\<^sub>l \<cdot> \<kappa> TrueV 
+      ELSE \<iota>\<^sub>r \<cdot> pred_expr \<parallel> pred_expr 
+      FI FI 
+        \<turnstile> Nat \<otimes> Nat \<rightarrow> Bool \<oplus> Nat \<otimes> Nat" by simp
+  qed
+
+lemma "greater_than_expr \<turnstile> Nat \<otimes> Nat \<rightarrow> Bool"
+  proof (unfold greater_than_expr_def)
+    have "\<lparr> \<Xi> \<rparr>\<^bsub>K Bool \<Oplus> funct.Id\<^esub> \<turnstile> \<mu> (K Bool \<Oplus> Id) \<rightarrow> Bool" by simp
+    moreover have "\<lbrakk> greater_than_helper \<rbrakk>\<^bsub>K Bool \<Oplus> Id\<^esub> \<turnstile> Nat \<otimes> Nat \<rightarrow> \<mu> (K Bool \<Oplus> Id)" by simp
+    ultimately show "\<lparr> \<Xi> \<rparr>\<^bsub>K Bool \<Oplus> funct.Id\<^esub> \<cdot> \<lbrakk> greater_than_helper \<rbrakk>\<^bsub>K Bool \<Oplus> Id\<^esub> 
+      \<turnstile> Nat \<otimes> Nat \<rightarrow> Bool" by (metis tc_comp)
+  qed
 
 lemma "length\<^bsub>t\<^esub> \<turnstile> List t \<rightarrow> Nat"
   proof (unfold length_expr_def)
@@ -24,8 +87,32 @@ primrec list_to_val :: "type \<Rightarrow> val list \<Rightarrow> val" where
 abbreviation long_run :: nat where
   "long_run \<equiv> Suc (Suc (Suc (Suc (Suc (Suc (Suc (Suc (Suc (Suc (Suc (Suc 0)))))))))))"
 
+lemma "partial_evaluation long_run is_zero_expr ZeroV = Some TrueV"
+  by (simp add: is_zero_expr_def)
+
+lemma "partial_evaluation long_run is_zero_expr (SuccV ZeroV) = Some FalseV"
+  by (simp add: is_zero_expr_def)
+
+lemma "partial_evaluation long_run is_zero_expr (SuccV (SuccV ZeroV)) = Some FalseV"
+  by (simp add: is_zero_expr_def)
+
+lemma "partial_evaluation long_run pred_expr ZeroV = Some ZeroV"
+  by (simp add: pred_expr_def)
+
+lemma "partial_evaluation long_run pred_expr (SuccV ZeroV) = Some ZeroV"
+  by (simp add: pred_expr_def)
+
+lemma "partial_evaluation long_run pred_expr (SuccV (SuccV ZeroV)) = Some (SuccV ZeroV)"
+  by (simp add: pred_expr_def)
+
 lemma "partial_evaluation long_run length\<^bsub>t\<^esub> (list_to_val t [a, b, c]) = 
     Some (nat_to_val (Suc (Suc (Suc 0))))"
   by (simp add: length_expr_def)
+
+lemma "partial_evaluation long_run greater_than_expr (PairV (SuccV (SuccV ZeroV)) (SuccV ZeroV)) = Some TrueV"
+  by (simp add: greater_than_expr_def greater_than_helper_def is_zero_expr_def pred_expr_def)
+
+lemma "partial_evaluation long_run greater_than_expr (PairV (SuccV ZeroV) (SuccV (SuccV ZeroV))) = Some FalseV"
+  by (simp add: greater_than_expr_def greater_than_helper_def is_zero_expr_def pred_expr_def)
 
 end
